update deps, remove enum wrapper struct, finish manual example

new_example/enum.go
@@ -1,6 +1,7 @@
 package main
 
 import (
+	"github.com/goose-lang/primitive"
 	"github.com/tchajed/marshal"
 )
 
@@ -13,54 +14,22 @@ const (
 	STATUS_PROFESSOR   Status = 3
 )
 
-type Person_Status struct {
-	status Status
-}
-
-func (ps *Person_Status) SetStatus(s Status) {
-	if s == STATUS_STUDENT {
-		ps.status = s
-	} else if s == STATUS_STAFF {
-		ps.status = s
-	} else if s == STATUS_PROFESSOR {
-		ps.status = s
-	} else {
-		ps.status = STATUS_UNSPECIFIED
-	}
-}
-
-func (ps *Person_Status) GetStatus() Status {
-	return ps.status
-}
-
-func MarshalPersonStatus(enc []byte, ps Person_Status) []byte {
-	enc = marshal.WriteInt(enc, uint64(ps.status))
-	return enc
-}
-
-func UnmarshalPersonStatus(s []byte) (Person_Status, []byte) {
-	status_int, s := marshal.ReadInt(s)
-	status := Person_Status{}
-	status.SetStatus(Status(status_int))
-	return status, s
-}
-
 type Person struct {
 	Name   string
-	Status Person_Status
+	Status Status
 }
 
 func MarshalPerson(enc []byte, p Person) []byte {
+	primitive.AssumeNoStringOverflow(p.Name)
 	enc = marshal.WriteLenPrefixedBytes(enc, []byte(p.Name))
-	enc = MarshalPersonStatus(enc, p.Status)
+	enc = marshal.WriteInt(enc, uint64(p.Status))
 	return enc
 }
 
 func UnmarshalPerson(s []byte) (Person, []byte) {
 	name, s := marshal.ReadLenPrefixedBytes(s)
 	status_int, s := marshal.ReadInt(s)
-	status := Person_Status{}
-	status.SetStatus(Status(status_int))
+	status := Status(status_int)
 
 	return Person{
 		Name:   string(name),
