new_example/pg/github_com/mjschwenne/grackle/new_example.v
@@ -88,74 +88,13 @@ Definition t := w64.
 End def.
 End Status.
 
-(* type main.Person_Status *)
-Module Person_Status.
-Section def.
-Context `{ffi_syntax}.
-Record t := mk {
-  status' : Status.t;
-}.
-End def.
-End Person_Status.
-
-Section instances.
-Context `{ffi_syntax}.
-
-Global Instance settable_Person_Status : Settable Person_Status.t :=
-  settable! Person_Status.mk < Person_Status.status' >.
-Global Instance into_val_Person_Status : IntoVal Person_Status.t :=
-  {| to_val_def v :=
-    struct.val_aux main.Person_Status [
-    "status" ::= #(Person_Status.status' v)
-    ]%struct
-  |}.
-
-Global Program Instance into_val_typed_Person_Status : IntoValTyped Person_Status.t main.Person_Status :=
-{|
-  default_val := Person_Status.mk (default_val _);
-|}.
-Next Obligation. solve_to_val_type. Qed.
-Next Obligation. solve_zero_val. Qed.
-Next Obligation. solve_to_val_inj. Qed.
-Final Obligation. solve_decision. Qed.
-
-Global Instance into_val_struct_field_Person_Status_status : IntoValStructField "status" main.Person_Status Person_Status.status'.
-Proof. solve_into_val_struct_field. Qed.
-
-
-Context `{!ffi_model, !ffi_semantics _ _, !ffi_interp _, !heapGS Σ}.
-Global Instance wp_struct_make_Person_Status status':
-  PureWp True
-    (struct.make #main.Person_Status (alist_val [
-      "status" ::= #status'
-    ]))%struct
-    #(Person_Status.mk status').
-Proof. solve_struct_make_pure_wp. Qed.
-
-
-Global Instance Person_Status_struct_fields_split dq l (v : Person_Status.t) :
-  StructFieldsSplit dq l v (
-    "Hstatus" ∷ l ↦s[main.Person_Status :: "status"]{dq} v.(Person_Status.status')
-  ).
-Proof.
-  rewrite /named.
-  apply struct_fields_split_intro.
-  unfold_typed_pointsto; split_pointsto_app.
-
-  rewrite -!/(typed_pointsto_def _ _ _) -!typed_pointsto_unseal.
-
-  solve_field_ref_f.
-Qed.
-
-End instances.
-
 (* type main.Person *)
 Module Person.
 Section def.
 Context `{ffi_syntax}.
 Record t := mk {
   Name' : go_string;
-  Status' : Person_Status.t;
+  Status' : Status.t;
 }.
 End def.
 End Person.
@@ -409,14 +348,6 @@ Global Instance wp_func_call_UnmarshalCalendar :
   WpFuncCall main "UnmarshalCalendar" _ (is_pkg_defined main) :=
   ltac:(apply wp_func_call'; reflexivity).
 
-Global Instance wp_func_call_MarshalPersonStatus :
-  WpFuncCall main "MarshalPersonStatus" _ (is_pkg_defined main) :=
-  ltac:(apply wp_func_call'; reflexivity).
-
-Global Instance wp_func_call_UnmarshalPersonStatus :
-  WpFuncCall main "UnmarshalPersonStatus" _ (is_pkg_defined main) :=
-  ltac:(apply wp_func_call'; reflexivity).
-
 Global Instance wp_func_call_MarshalPerson :
   WpFuncCall main "MarshalPerson" _ (is_pkg_defined main) :=
   ltac:(apply wp_func_call'; reflexivity).
@@ -440,14 +371,6 @@ Global Instance wp_func_call_MarshalTimeStamp :
 Global Instance wp_func_call_UnmarshalTimeStamp :
   WpFuncCall main "UnmarshalTimeStamp" _ (is_pkg_defined main) :=
   ltac:(apply wp_func_call'; reflexivity).
-
-Global Instance wp_method_call_Person_Status'ptr_GetStatus :
-  WpMethodCall main "Person_Status'ptr" "GetStatus" _ (is_pkg_defined main) :=
-  ltac:(apply wp_method_call'; reflexivity).
-
-Global Instance wp_method_call_Person_Status'ptr_SetStatus :
-  WpMethodCall main "Person_Status'ptr" "SetStatus" _ (is_pkg_defined main) :=
-  ltac:(apply wp_method_call'; reflexivity).
 
 End names.
 End main.
